Use upto technique for adq proof

specIR/SimSIR.v
@@ -29,122 +29,462 @@ Set Implicit Arguments.
 
 Local Obligation Tactic := ii; ss; eauto.
 
+Definition hrespectful A0 A1 B0 B1 (RA: A0 -> A1 -> Prop) (RB: B0 -> B1 -> Prop):
+  (A0 -> B0) -> (A1 -> B1) -> Prop :=
+  fun f0 f1 => forall a0 a1, RA a0 a1 -> RB (f0 a0) (f1 a1)
+.
+
+Definition hrespectful_respectful A B (RA: relation A) (RB: relation B):
+  @hrespectful A A B B RA RB = @respectful A B RA RB.
+Proof. ss. Qed.
+
+Notation " R **> R' " := (@hrespectful _ _ _ _ (R%signature) (R'%signature))
+                           (right associativity, at level 55).
+                         (* : signature_scope. *)
+
+Class HProper A0 A1 (R : A0 -> A1 -> Prop) (a0: A0) (a1: A1) : Prop := hproper_prf : R a0 a1.
+
+Program Instance HProper_Proper A RA (a: A) (P: HProper RA a a): Proper RA a.
+
+Hint Unfold hrespectful.
+Hint Unfold HProper.
+(**
+Ltac uh := unfold hrespectful in *; unfold HProper in *.
+Tactic Notation "uh" "in" hyp(H) := repeat (autounfold with * in H; cbn in H).
+Tactic Notation "u" := repeat (autounfold with *; cbn).
+Tactic Notation "u" "in" "*" := repeat (autounfold with * in *; cbn in * ).
+**)
+
+
+
+(*** TODO: move to SIRCommon ***)
+Lemma unfold_interp_mrec :
+forall (D E : Type -> Type) (ctx : forall T : Type, D T -> itree (D +' E) T) 
+  (R : Type) (t : itree (D +' E) R), interp_mrec ctx t = _interp_mrec ctx (observe t).
+Proof.
+  i. f. eapply unfold_interp_mrec; et.
+Qed.
+
+Lemma bind_ret_l : forall (E : Type -> Type) (R S : Type) (r : R) (k : R -> itree E S),
+    ` x : _ <- Ret r;; k x = k r.
+Proof.
+  i. f. eapply bind_ret_l.
+Qed.
+
+Lemma bind_ret_r : forall (E : Type -> Type) (R : Type) (s : itree E R), ` x : R <- s;; Ret x = s.
+Proof.
+  i. f. eapply bind_ret_r.
+Qed.
+
+Lemma bind_tau : forall (E : Type -> Type) (R U : Type) (t : itree E U) (k : U -> itree E R),
+  ` x : _ <- Tau t;; k x = Tau (` x : _ <- t;; k x).
+Proof.
+  i. f. eapply bind_tau.
+Qed.
+
+Lemma bind_vis: forall (E : Type -> Type) (R U V : Type) (e : E V) (ek : V -> itree E U) (k : U -> itree E R),
+  ` x : _ <- Vis e ek;; k x = Vis e (fun x : V => ` x : _ <- ek x;; k x).
+Proof.
+  i. f. eapply bind_vis.
+Qed.
+
+
+
+
+
 Section OWNEDHEAP.
 
 Variable mi: string.
-Variable owned_heap0 owned_heap1: Type.
-Variable SO: owned_heap0 -> owned_heap1 -> Prop.
-
-
-Let ktr0 := function owned_heap0.
-Let ktr1 := function owned_heap1.
-Let itr0 := itree (E owned_heap0) (owned_heap0 * (mem * val)).
-Let itr1 := itree (E owned_heap1) (owned_heap1 * (mem * val)).
-
-
-(**************** TODO: eqit is defined in terms of "itree'", not "itree" *****************)
-
-
-(* Variable fname: ident. *)
-(* Variable oh0: owned_heap0. *)
-(* Variable m0: mem. *)
-(* Variable vs0: list val. *)
-(* Check (ICall fname oh0 m0 vs0). *)
-(* Variable k0: ((owned_heap0 * (mem * val)) -> itr0). *)
-(* Check (Vis (subevent _ (ICall fname oh0 m0 vs0)) k0). *)
-
-
-Inductive _sim_itr (sim_itr: itr0 -> itr1 -> Prop): itr0 -> itr1 -> Prop :=
-| sim_ret
-    oh0 oh1 m v
-  :
-    _sim_itr sim_itr (Ret (oh0, (m, v))) (Ret (oh1, (m, v)))
-| sim_tau
-    i0
-    i1
-    (SIM: sim_itr i0 i1)
-  :
-    _sim_itr sim_itr (Tau i0) (Tau i1)
-| sim_icall
-    fname m vs
-    oh0 k0
-    oh1 k1
-    (SIM: forall
-        mr vr
-        ohr0
-        ohr1
-      ,
-        sim_itr (k0 (ohr0, (mr, vr))) (k1 (ohr1, (mr, vr))))
-  :
-    _sim_itr sim_itr
-             (Vis (subevent _ (ICall fname oh0 m vs)) k0)
-             (Vis (subevent _ (ICall fname oh1 m vs)) k1)
-| sim_ecall
-    sg m vs
-    fptr0 oh0 k0
-    fptr1 oh1 k1
-    (SIM: forall
-        mr vr
-        ohr0 ohr1
-      ,
-        sim_itr (k0 (ohr0, (mr, vr))) (k1 (ohr1, (mr, vr))))
-  :
-    _sim_itr sim_itr
-             (Vis (subevent _ (ECall sg fptr0 oh0 m vs)) k0)
-             (Vis (subevent _ (ECall sg fptr1 oh1 m vs)) k1)
-| sim_nb
-    i0 k1
-  :
-    _sim_itr sim_itr i0 (Vis (subevent _ (ENB)) k1)
-| sim_ub
-    k0 i1
-  :
-    _sim_itr sim_itr (Vis (subevent _ (ENB)) k0) i1
-| sim_choose_src
-    X0
-    k0 i1
-    (SIM: exists x0, sim_itr (k0 x0) i1)
-  :
-    _sim_itr sim_itr
-             (Vis (subevent _ (EChoose X0)) k0)
-             (Tau i1)
-| sim_choose_tgt
-    X1
-    k1 i0
-    (SIM: forall x1, sim_itr i0 (k1 x1))
-  :
-    _sim_itr sim_itr
-             (Tau i0)
-             (Vis (subevent _ (EChoose X1)) k1)
+Variable owned_heap_src owned_heap_tgt: Type.
+Variable SO: owned_heap_src -> owned_heap_tgt -> Prop.
+Definition SALL: (owned_heap_src * (mem * val)) -> (owned_heap_tgt * (mem * val)) -> Prop :=
+  fun '(oh_src, (m_src, vs_src)) '(oh_tgt, (m_tgt, vs_tgt)) =>
+    <<O: SO oh_src oh_tgt>> /\ <<M: m_src = m_tgt>> /\ <<VS: vs_src = vs_tgt>>
 .
 
-Definition sim_itr: itr0 -> itr1 -> Prop := paco2 _sim_itr bot2.
+
+
+
+
+(*** sim syntax ***)
+Section SYNTAX.
+
+(*** sim itree ***)
+Let itr_src := itree (E owned_heap_src) (owned_heap_src * (mem * val)).
+Let itr_tgt := itree (E owned_heap_tgt) (owned_heap_tgt * (mem * val)).
+
+Inductive _sim_itr (sim_itr: itr_src -> itr_tgt -> Prop): itr_src -> itr_tgt -> Prop :=
+| sim_ret
+    oh_src oh_tgt m v
+    (O: SO oh_src oh_tgt)
+  :
+    _sim_itr sim_itr (Ret (oh_src, (m, v))) (Ret (oh_tgt, (m, v)))
+| sim_tau
+    i_src
+    i_tgt
+    (SIM: sim_itr i_src i_tgt)
+  :
+    _sim_itr sim_itr (Tau i_src) (Tau i_tgt)
+| sim_icall
+    fname m vs
+    oh_src k_src
+    oh_tgt k_tgt
+    (O: SO oh_src oh_tgt)
+    (SIM: HProper (SALL **> sim_itr) k_src k_tgt)
+    (* (SIM: forall *)
+    (*     mr vr *)
+    (*     ohr_src *)
+    (*     ohr_tgt *)
+    (*   , *)
+    (*     sim_itr (k_src (ohr_src, (mr, vr))) (k_tgt (ohr_tgt, (mr, vr)))) *)
+  :
+    _sim_itr sim_itr
+             (Vis (subevent _ (ICall fname oh_src m vs)) k_src)
+             (Vis (subevent _ (ICall fname oh_tgt m vs)) k_tgt)
+| sim_ecall
+    sg m vs
+    fptr_src oh_src k_src
+    fptr_tgt oh_tgt k_tgt
+    (O: SO oh_src oh_tgt)
+    (SIM: HProper (SALL **> sim_itr) k_src k_tgt)
+    (* (SIM: forall *)
+    (*     mr vr *)
+    (*     ohr_src ohr_tgt *)
+    (*   , *)
+    (*     sim_itr (k_src (ohr_src, (mr, vr))) (k_tgt (ohr_tgt, (mr, vr)))) *)
+  :
+    _sim_itr sim_itr
+             (Vis (subevent _ (ECall sg fptr_src oh_src m vs)) k_src)
+             (Vis (subevent _ (ECall sg fptr_tgt oh_tgt m vs)) k_tgt)
+| sim_nb
+    i_src k_tgt
+  :
+    _sim_itr sim_itr i_src (Vis (subevent _ (ENB)) k_tgt)
+| sim_ub
+    k_src i_tgt
+  :
+    _sim_itr sim_itr (Vis (subevent _ (ENB)) k_src) i_tgt
+| sim_choose_src
+    X_src
+    k_src i_tgt
+    (SIM: exists x_src, sim_itr (k_src x_src) i_tgt)
+  :
+    _sim_itr sim_itr
+             (Vis (subevent _ (EChoose X_src)) k_src)
+             (Tau i_tgt)
+| sim_choose_tgt
+    X_tgt
+    k_tgt i_src
+    (SIM: forall x_tgt, sim_itr i_src (k_tgt x_tgt))
+  :
+    _sim_itr sim_itr
+             (Tau i_src)
+             (Vis (subevent _ (EChoose X_tgt)) k_tgt)
+.
+
+Definition sim_itr: itr_src -> itr_tgt -> Prop := paco2 _sim_itr bot2.
 
 Lemma sim_itr_mon: monotone2 _sim_itr.
 Proof.
-  ii. inv IN; try econs; et.
+  ii. inv IN; try econs; et; rr; et.
   des. esplits; et.
 Unshelve.
 Qed.
 Hint Unfold sim_itr.
 Hint Resolve sim_itr_mon: paco.
 
-Definition sim_ktr (k0: ktr0) (k1: ktr1): Prop := forall
+
+
+(*** sim fn ***)
+Let fn_src := function owned_heap_src.
+Let fn_tgt := function owned_heap_tgt.
+
+(*** TODO: curry "function", and we can state "SALL **> sim_itr ***)
+(*** TODO: give better name than SALL ***)
+Definition sim_fn (k_src: fn_src) (k_tgt: fn_tgt): Prop := forall
     m vs
-    oh0 oh1
-    (O: SO oh0 oh1)
+    oh_src oh_tgt
+    (O: SO oh_src oh_tgt)
   ,
-    <<SIM: sim_itr (k0 oh0 m vs) (k1 oh1 m vs)>>
+    <<SIM: sim_itr (k_src oh_src m vs) (k_tgt oh_tgt m vs)>>
 .
 
 
 
 
-(*** Lifting to SimModSem ***)
 
-Definition sim_prog (p0: program owned_heap0) (p1: program owned_heap1): Prop :=
-  forall fname, <<SIM: option_rel sim_ktr (p0 fname) (p1 fname)>>
+(*** sim prog ***)
+Definition sim_prog (p_src: program owned_heap_src) (p_tgt: program owned_heap_tgt): Prop :=
+  forall fname, option_rel sim_fn (p_src fname) (p_tgt fname)
 .
+
+
+
+
+(*** useful lemma for below proof ***)
+(*** copied from "eqit_bind_clo" in itree repo - Eq.v ***)
+Inductive bindC (r: itr_src -> itr_tgt -> Prop) : itr_src -> itr_tgt -> Prop :=
+| bindC_intro
+    i_src i_tgt
+    (SIM: sim_itr i_src i_tgt)
+    k_src k_tgt
+    (SIMK: HProper (SALL **> r) k_src k_tgt)
+    (* (SIMK: forall *)
+    (*     oh_src oh_tgt m vs *)
+    (*     (O: SO oh_src oh_tgt) *)
+    (*   , *)
+    (*     <<SIM: r (k_src (oh_src, (m, vs))) (k_tgt (oh_tgt, (m, vs)))>>) *)
+  :
+    bindC r (ITree.bind i_src k_src) (ITree.bind i_tgt k_tgt)
+.
+
+Hint Constructors bindC: core.
+
+Lemma bindC_spec
+      simC
+  :
+    bindC <3= gupaco2 (_sim_itr) (simC)
+.
+Proof.
+  gcofix CIH. intros. destruct PR.
+  punfold SIM. inv SIM.
+  - rewrite ! bind_ret_l. gbase. eapply SIMK; et. rr; et.
+  - rewrite ! bind_tau. gstep. econs; eauto. pclearbot.
+    (* gfinal. left. eapply CIH. econstructor; eauto. *)
+    debug eauto with paco.
+  - rewrite ! bind_vis. gstep. econs; eauto. u. ii. repeat spc SIM0. pclearbot.
+    (* gfinal. left. eapply CIH. econs. { et. } uh. ii. eapply SIMK. et. *)
+    eauto with paco.
+  - rewrite ! bind_vis. gstep. econs; eauto. u. ii. repeat spc SIM0. pclearbot.
+    eauto with paco.
+  - rewrite ! bind_vis. gstep. econs; eauto.
+  - rewrite ! bind_vis. gstep. econs; eauto.
+  - rewrite ! bind_vis. rewrite ! bind_tau.
+    gstep. econs; eauto. des. pclearbot. eauto with paco.
+  - rewrite ! bind_vis. rewrite ! bind_tau.
+    gstep. econs; eauto. ii. pclearbot. eauto with paco.
+Qed.
+
+Global Instance sim_itr_bind :
+  HProper ((SALL **> sim_itr) **> sim_itr **> sim_itr) ITree.bind' ITree.bind'
+.
+Proof.
+  red. ginit.
+  { intros. eapply cpn2_wcompat; eauto with paco. }
+  guclo bindC_spec. ii. econs; et.
+  u. ii.
+  exploit H0; et.
+  intro T. eauto with paco.
+Qed.
+
+End SYNTAX.
+Hint Unfold sim_itr.
+Hint Resolve sim_itr_mon: paco.
+
+
+
+
+
+
+
+
+
+(*** sim semantics ***)
+Section SEMANTICS.
+
+(*** sim states ***)
+Let st_src := (SIRmini.state owned_heap_src).
+Let st_tgt := (SIRmini.state owned_heap_tgt).
+
+Inductive _sim_st (sim_st: st_src -> st_tgt -> Prop): st_src -> st_tgt -> Prop :=
+| sim_st_ret
+    oh_src oh_tgt m v
+    (O: SO oh_src oh_tgt)
+  :
+    _sim_st sim_st (Ret (oh_src, (m, v))) (Ret (oh_tgt, (m, v)))
+| sim_st_tau
+    i_src
+    i_tgt
+    (SIM: sim_st i_src i_tgt)
+  :
+    _sim_st sim_st (Tau i_src) (Tau i_tgt)
+| sim_st_ecall
+    sg m vs
+    fptr_src oh_src k_src
+    fptr_tgt oh_tgt k_tgt
+    (O: SO oh_src oh_tgt)
+    (SIM: HProper (SALL **> sim_st) k_src k_tgt)
+  :
+    _sim_st sim_st
+             (Vis (subevent _ (ECall sg fptr_src oh_src m vs)) k_src)
+             (Vis (subevent _ (ECall sg fptr_tgt oh_tgt m vs)) k_tgt)
+| sim_st_nb
+    i_src k_tgt
+  :
+    _sim_st sim_st i_src (Vis (subevent _ (ENB)) k_tgt)
+| sim_st_ub
+    k_src i_tgt
+  :
+    _sim_st sim_st (Vis (subevent _ (ENB)) k_src) i_tgt
+| sim_st_choose_src
+    X_src
+    k_src i_tgt
+    (SIM: exists x_src, sim_st (k_src x_src) i_tgt)
+  :
+    _sim_st sim_st
+            (Vis (subevent _ (EChoose X_src)) k_src)
+            i_tgt 
+| sim_st_choose_tgt
+    X_tgt
+    k_tgt i_src
+    (SIM: forall x_tgt, sim_st i_src (k_tgt x_tgt))
+  :
+    _sim_st sim_st
+            i_src
+            (Vis (subevent _ (EChoose X_tgt)) k_tgt)
+.
+
+Definition sim_st: st_src -> st_tgt -> Prop := paco2 _sim_st bot2.
+
+Lemma sim_st_mon: monotone2 _sim_st.
+Proof.
+  ii. inv IN; try econs; et.
+  des. esplits; et.
+Unshelve.
+Qed.
+Hint Unfold sim_st.
+Hint Resolve sim_st_mon: paco.
+
+End SEMANTICS.
+Hint Unfold sim_st.
+Hint Resolve sim_st_mon: paco.
+
+
+
+
+
+
+
+
+
+Lemma sim_prog_sim_st_aux
+      p_src p_tgt
+      (SIMP: sim_prog p_src p_tgt)
+      i_src i_tgt
+      (SIM: sim_itr i_src i_tgt)
+  :
+    sim_st (interp_mrec (interp_function p_src) i_src) (interp_mrec (interp_function p_tgt) i_tgt)
+.
+Proof.
+  revert_until SIMP.
+  ginit.
+  { intros. eapply cpn2_wcompat; et. eauto with paco. }
+  gcofix CIH.
+  i. rewrite ! unfold_interp_mrec.
+  punfold SIM. inv SIM; cbn.
+  - gstep. econs; et.
+  - pclearbot. gstep. econs; et. gbase. et.
+  - pclearbot. gstep. econs; et. gbase.
+    eapply CIH. eapply sim_itr_bind.
+    { u. ii. repeat spc SIM0. pclearbot. eauto. }
+    hexploit (SIMP fname); et. intro T.
+    inv T.
+    { pfold. econs; et. }
+    exploit H1; et.
+  - gstep. econs; et. u in *. gstep. econs; et. repeat spc SIM0. des; ss. gbase. eapply CIH.
+    eauto with paco.
+  - gstep. econs; et.
+  - gstep. econs; et.
+  - gstep. des. pclearbot. econs; et. esplits; et. gstep. econs; et. eauto with paco.
+  - gstep. pclearbot. econs; et. ii. repeat spc SIM0.
+    gstep. econs; et. eauto with paco.
+Qed.
+
+Theorem sim_prog_sim_st
+        p_src p_tgt
+        (SIMP: sim_prog p_src p_tgt)
+  :
+    forall
+      (fname: ident) m vs oh_src oh_tgt
+      (O: SO oh_src oh_tgt)
+    ,
+      (<<SIM: sim_st (interp_program0 p_src (ICall fname oh_src m vs))
+                     (interp_program0 p_tgt (ICall fname oh_tgt m vs))
+                     >>)
+.
+Proof.
+  {
+    ii.
+    eapply sim_prog_sim_st_aux; ss.
+    hexploit (SIMP fname); et. intro T. inv T; ss.
+    { pfold. econs; et. }
+    repeat (spc H1). des. ss.
+  }
+Qed.
+
+
+(*** sim fn / program ***)
+(* Let fn_src := InternalCallE owned_heap_src ~> SIRmini.state. *)
+(* Let fn_tgt := InternalCallE owned_heap_tgt ~> SIRmini.state. *)
+
+(* Definition sim_fn (k_src: fn_src) (k_tgt: fn_tgt): Prop := forall *)
+(*     fname m vs *)
+(*     oh_src oh_tgt *)
+(*     (O: SO oh_src oh_tgt) *)
+(*   , *)
+(*     <<SIM: sim_st (k_src _ (ICall fname oh_src m vs)) (k_tgt _ (ICall fname oh_tgt m vs))>> *)
+(* . *)
+Let fn_src := function owned_heap_src.
+Let fn_tgt := function owned_heap_tgt.
+
+Definition sim_fn (k_src: fn_src) (k_tgt: fn_tgt): Prop := forall
+    m vs
+    oh_src oh_tgt
+    (O: SO oh_src oh_tgt)
+  ,
+    <<SIM: sim_st (k_src oh_src m vs) (k_tgt oh_tgt m vs)>>
+.
+
+Definition sim_prog (p_src: program owned_heap_src) (p_tgt: program owned_heap_tgt): Prop :=
+  (eq ===> 
+.
+Definition sim_prog (p_src: program owned_heap_src) (p_tgt: program owned_heap_tgt): Prop :=
+  forall fname, <<SIM: option_rel sim_fn (p_src fname) (p_tgt fname)>>
+.
+
+Theorem sim_prog_sim_st
+        p_src p_tgt
+        (SIM: sim_prog p_src p_tgt)
+  :
+    <<SIM: sim_ktr (interp_program0 p_src) (interp_program0 p_tgt)>>
+.
+Proof.
+Qed.
+Global Instance eq_itree_mrec:
+  Proper (sim_prog ==> eq ==> sim_st) (interp_program0).
+Proof.
+  ginit. gcofix CIH. intros.
+  rewrite !unfold_interp_mrec.
+  punfold H0. inv H0; try discriminate; pclearbot; simpobs; [| |destruct e]; gstep.
+  - apply reflexivity.
+  - econstructor. eauto with paco.
+  - econstructor. gbase. eapply CIH. apply eqit_bind; auto; reflexivity.
+  - econstructor. gstep; constructor. auto with paco.
+Qed.
+
+Theorem sim_sim
+        
+
+
+
+
+
+
+
+
+
+
+
 
 
 
@@ -160,9 +500,9 @@ Section SMO.
 
   Inductive wf (smo: t): Prop :=
   | wf_intro
-      (oh0: owned_heap0) (oh1: owned_heap1)
+      (oh_src: owned_heap_src) (oh1: owned_heap1)
       (MWF: SimMem.wf smo)
-      (OHSRC: smo.(oh_src) = upcast oh0)
+      (OHSRC: smo.(oh_src) = upcast oh_src)
       (OHTGT: smo.(oh_tgt) = upcast oh1)
   .
 
@@ -189,25 +529,26 @@ Section SMO.
     econs; ss; et.
   Qed.
   Next Obligation.
-    ss. ii. destruct smo0; ss.
+    ss. ii. destruct smo_src; ss.
   Qed.
 
 End SMO.
 
 
 
-Variable p0: program owned_heap0.
+Variable p_src: program owned_heap_src.
 Variable p1: program owned_heap1.
-Variable ioh0: SkEnv.t -> owned_heap0.
+Variable ioh_src: SkEnv.t -> owned_heap_src.
 Variable ioh1: SkEnv.t -> owned_heap1.
-Hypothesis (SIMP: sim_prog p0 p1).
-Hypothesis (SIMO: forall skenv, SO (ioh0 skenv) (ioh1 skenv)).
+Hypothesis (SIMP: sim_prog p_src p1).
+Hypothesis (SIMO: forall skenv, SO (ioh_src skenv) (ioh1 skenv)).
 Variable sk: Sk.t.
-Let md_src: Mod.t := (SIRmini.module sk p0 mi ioh0).
+Let md_src: Mod.t := (SIRmini.module sk p_src mi ioh_src).
 Let md_tgt: Mod.t := (SIRmini.module sk p1 mi ioh1).
 
 
 
+(*** Lifting to SimModSem ***)
 Section SIMMODSEM.
 
 Variable skenv_link: SkEnv.t.
@@ -223,17 +564,17 @@ Local Arguments ModSemPair.mk [SM] [SS] _ _ _ _ [SMO].
 Definition msp: ModSemPair.t := ModSemPair.mk (md_src skenv_link) (md_tgt skenv_link)
                                               (SimSymbId.mk md_src md_tgt) sm_link.
 
-Inductive match_states (idx: nat): SIRmini.state owned_heap0 ->
+Inductive match_states (idx: nat): SIRmini.state owned_heap_src ->
                                    SIRmini.state owned_heap1 -> SimMemOh.t -> Prop :=
 | match_states_intro
-    st0 st1 smo0
-    fid m vs oh0 oh1
-    (O: SO oh0 oh1)
-    (ST0: st0 = (interp_program0 p0 (ICall fid oh0 m vs)))
-    (ST1: st1 = (interp_program0 p1 (ICall fid oh1 m vs)))
-    (MWF: SimMemOh.wf smo0)
+    st_src st1 smo_src
+    fid m vs oh_src oh1
+    (O: SO oh_src oh1)
+    (ST_src: st_src = (interp_program_src p_src (ICall fid oh_src m vs)))
+    (ST1: st1 = (interp_program_src p1 (ICall fid oh1 m vs)))
+    (MWF: SimMemOh.wf smo_src)
   :
-    match_states idx st0 st1 smo0
+    match_states idx st_src st1 smo_src
 .
 
 (*** TODO: move to SIRCommon2 ***)
@@ -245,12 +586,12 @@ Proof.
 Qed.
 
 Lemma match_states_lxsim
-      idx st_src0 st_tgt0 smo0
-      (MATCH: match_states idx st_src0 st_tgt0 smo0)
+      idx st_src_src st_tgt_src smo_src
+      (MATCH: match_states idx st_src_src st_tgt_src smo_src)
   :
     <<XSIM: lxsim (md_src skenv_link) (md_tgt skenv_link)
                   (fun _ => () -> exists (_ : ()) (_ : mem), True)
-                  (Ord.lift_idx lt_wf idx) st_src0 st_tgt0 smo0>>
+                  (Ord.lift_idx lt_wf idx) st_src_src st_tgt_src smo_src>>
 .
 Proof.
   revert_until idx. revert idx.
@@ -259,8 +600,8 @@ Proof.
 
   inv MATCH. ss.
   hexploit (SIMP fid); et. intro R.
-  unfold interp_program0, mrec in *.
-  (* f in ST0. rewrite unfold_interp_mrec in ST0. ss. *)
+  unfold interp_program_src, mrec in *.
+  (* f in ST_src. rewrite unfold_interp_mrec in ST_src. ss. *)
   inv R; des_ifs; ss.
   { des_ifs. rewrite ! unfold_interp_mrec. ss. econs 2; eauto. ii. econs 3; et.
     { ss. ii. inv STEPTGT; ss. }
@@ -269,10 +610,10 @@ Proof.
   des_ifs.
   rename H1 into SK.
   exploit (SK m vs); et. intro SI. des.
-  rewrite ! unfold_interp_mrec. rename f0 into f1. rename f into f0.
+  rewrite ! unfold_interp_mrec. rename f_src into f1. rename f into f_src.
   punfold SI. inv SI.
   - (* RET *)
-    econstructor 4 with (smo_ret := mk (SimMemId.mk m0 m0) (upcast oh2) (upcast oh3)); ss; eauto.
+    econstructor 4 with (smo_ret := mk (SimMemId.mk m_src m_src) (upcast oh2) (upcast oh3)); ss; eauto.
     { econs; ss; et. }
     { econs; ss; et. }
     { econs; ss; et. }
@@ -295,13 +636,13 @@ Qed.
 End SIMMODSEM.
 
 Theorem sim_mod
-        p0 p1
-        ioh0 ioh1
-        (SIMP: sim_prog p0 p1)
-        (SIMO: forall skenv, SO (ioh0 skenv) (ioh1 skenv))
+        p_src p1
+        ioh_src ioh1
+        (SIMP: sim_prog p_src p1)
+        (SIMO: forall skenv, SO (ioh_src skenv) (ioh1 skenv))
   :
     forall sk,
-      ModPair.sim (SimSymbId.mk_mp (SIRmini.module sk p0 mi ioh0) (SIRmini.module sk p1 mi ioh1))
+      ModPair.sim (SimSymbId.mk_mp (SIRmini.module sk p_src mi ioh_src) (SIRmini.module sk p1 mi ioh1))
 .
 Proof.
   ii. econs; ss; eauto.
